Wavelet/Determinacy/Congr.lean
@@ -1,0 +1,116 @@
+import Wavelet.Determinacy.Defs
+import Wavelet.Determinacy.Determinism
+
+/-! Lemmas about converting steps through `EqMod`. -/
+
+namespace Wavelet.Dataflow
+
+open Semantics Determinacy
+
+theorem async_op_interp_congr
+  [InterpConsts V]
+  {aop aop' aop₁ aop₁' : AsyncOp (V ⊕ T)}
+  (hinterp : AsyncOp.Interp aop
+    (.mk allInputs allOutputs inputs inputVals outputs outputVals) aop₁)
+  (heq_aop : AsyncOp.EqMod EqModGhost aop aop')
+  (heq_inputs : List.Forall₂ EqModGhost inputVals inputVals') :
+    ∃ outputVals',
+      AsyncOp.Interp aop'
+        (.mk allInputs allOutputs inputs inputVals' outputs outputVals') aop₁' ∧
+      AsyncOp.EqMod EqModGhost aop₁ aop₁' ∧
+      List.Forall₂ EqModGhost outputVals outputVals'
+  := sorry
+
+theorem proc_indexed_unguarded_congr
+  [Arity Op]
+  [DecidableEq χ]
+  [InterpConsts V]
+  {opSpec : OpSpec Op V T}
+  {s₁ s₁' s₂ : ConfigWithSpec opSpec χ m n}
+  {l : Nat × Label Op V m n}
+  (hstep : (Config.IdxTrivStep opSpec).Step s₁ l s₂)
+  (heq : Config.EqMod EqModGhost s₁ s₁') :
+    ∃ s₂',
+      (Config.IdxTrivStep opSpec).Step s₁' l s₂' ∧
+      Config.EqMod EqModGhost s₂ s₂'
+  := by
+  have hl := proc_indexed_unguarded_step_label hstep
+  have ⟨heq_aps, heq_chans⟩ := heq
+  rcases hstep with ⟨⟨hguard⟩, hstep⟩
+  cases hstep with
+  | step_op => sorry
+  | step_async hi hget hinterp hpop => sorry
+    -- replace ⟨_, _, hpop, heq_outputs, heq_chans'⟩ := chan_map_pop_vals_equiv heq_chans hpop
+    -- -- simp at hpop
+    -- exact ⟨
+    --   _,
+    --   .step
+    --     (.idx_guard hguard)
+    --     (.step_async
+    --       hi
+    --       hget
+    --       hinterp
+    --       hpop),
+    --   sorry
+    -- ⟩
+
+theorem proc_indexed_interp_unguarded_congr
+  [Arity Op]
+  [DecidableEq χ]
+  [InterpConsts V]
+  [opInterp : OpInterp Op V]
+  {opSpec : OpSpec Op V T}
+  {s₁ s₁' s₂ : ConfigWithSpec opSpec χ m n × opInterp.S}
+  (hstep : (Config.IdxInterpTrivStep opSpec).Step s₁ l s₂)
+  (heq : Config.EqMod EqModGhost s₁.1 s₁'.1 ∧ s₁.2 = s₁'.2) :
+    ∃ s₂',
+      (Config.IdxInterpTrivStep opSpec).Step s₁' l s₂' ∧
+      Config.EqMod EqModGhost s₂.1 s₂'.1 ∧
+      s₂.2 = s₂'.2
+  := by
+  have hl := proc_indexed_interp_unguarded_step_label hstep
+  cases hstep with
+  | step_yield hstep hinterp =>
+    have ⟨_, hstep', heq'⟩ := proc_indexed_unguarded_congr hstep heq.1
+    simp at heq
+    simp [heq.2] at hinterp
+    exact ⟨
+      _, .step_yield hstep' hinterp,
+      by
+        simp at heq ⊢
+        simp [heq']
+    ⟩
+  | step_tau hstep =>
+    have ⟨_, hstep', heq'⟩ := proc_indexed_unguarded_congr hstep heq.1
+    exact ⟨
+      _, .step_tau hstep',
+      by
+        simp at heq ⊢
+        simp [heq, heq']
+    ⟩
+  | _ hstep => simp at hl
+
+theorem proc_indexed_interp_unguarded_steps_congr
+  [Arity Op]
+  [DecidableEq χ]
+  [InterpConsts V]
+  [opInterp : OpInterp Op V]
+  {opSpec : OpSpec Op V T}
+  {s₁ s₁' s₂ : ConfigWithSpec opSpec χ m n × opInterp.S}
+  (htrace : (Config.IdxInterpTrivStep opSpec).Star s₁ tr s₂)
+  (heq : Config.EqMod EqModGhost s₁.1 s₁'.1 ∧ s₁.2 = s₁'.2) :
+    ∃ s₂',
+      (Config.IdxInterpTrivStep opSpec).Star s₁' tr s₂' ∧
+      Config.EqMod EqModGhost s₂.1 s₂'.1 ∧
+      s₂.2 = s₂'.2
+  := by
+  induction htrace
+    using Lts.Star.reverse_induction
+    generalizing s₁' with
+  | refl => exact ⟨s₁', .refl, heq⟩
+  | head hstep htail ih =>
+    have ⟨_, hstep', heq₁⟩ := proc_indexed_interp_unguarded_congr hstep heq
+    have ⟨_, htail', heq₂⟩ := ih heq₁
+    exact ⟨_, htail'.prepend hstep', heq₂⟩
+
+end Wavelet.Dataflow
