Wavelet/Determinacy/Convert.lean
@@ -1,0 +1,143 @@
+import Wavelet.Determinacy.Defs
+
+/-! Conversion between various stepping relations. -/
+
+namespace Wavelet.Determinacy
+
+open Semantics Dataflow
+
+/-- Converts an indexed guarded step to a guarded step. -/
+theorem proc_indexed_guarded_step_to_guarded_step
+  [Arity Op] [PCM T]
+  [DecidableEq χ]
+  [InterpConsts V]
+  {opSpec : OpSpec Op V T}
+  {ioSpec : IOSpec V T m n}
+  {s s' : ConfigWithSpec opSpec χ m n}
+  {l : Label Op V m n}
+  (hl : l.isYield ∨ l.isSilent)
+  (hstep : (Config.IdxGuardStep opSpec ioSpec).Step s (i, l) s') :
+    (Config.GuardStep opSpec ioSpec) s l s'
+  := by
+  rcases hstep with ⟨⟨hguard⟩, hstep⟩
+  cases hguard <;> simp at hl
+  case spec_yield =>
+    have := Config.IndexedStep.to_step_yield_or_tau hstep
+    exact .step .spec_yield this
+  case spec_join h₁ h₂ h₃ =>
+    have := Config.IndexedStep.to_step_yield_or_tau hstep
+    exact .step (.spec_join h₁ h₂ h₃) this
+  case spec_tau =>
+    have := Config.IndexedStep.to_step_yield_or_tau hstep
+    exact .step .spec_tau this
+
+/-- Converts a guarded step to an indexed guarded step. -/
+theorem proc_guarded_step_to_indexed_guarded_step
+  [Arity Op] [PCM T]
+  [DecidableEq χ]
+  [InterpConsts V]
+  {opSpec : OpSpec Op V T}
+  {ioSpec : IOSpec V T m n}
+  {s s' : ConfigWithSpec opSpec χ m n}
+  {l : Label Op V m n}
+  (hl : l.isYield ∨ l.isSilent)
+  (hstep : (Config.GuardStep opSpec ioSpec) s l s') :
+    ∃ i, (Config.IdxGuardStep opSpec ioSpec).Step s (i, l) s'
+  := by
+  cases hstep with | step hguard hstep
+  cases hguard <;> simp at hl
+  case step.spec_yield =>
+    have ⟨i, hstep'⟩ := Config.IndexedStep.from_step_yield hstep
+    exact ⟨i, .step (.idx_guard .spec_yield) hstep'⟩
+  case step.spec_join h₁ h₂ h₃ =>
+    have ⟨i, hstep'⟩ := Config.IndexedStep.from_step_yield hstep
+    exact ⟨i, .step (.idx_guard (.spec_join h₁ h₂ h₃)) hstep'⟩
+  case step.spec_tau =>
+    have ⟨i, hstep'⟩ := Config.IndexedStep.from_step_tau hstep
+    exact ⟨i, .step (.idx_guard .spec_tau) hstep'⟩
+
+/-- Converts an indexed unguarded step to an unguarded step. -/
+theorem proc_indexed_unguarded_step_to_unguarded_step
+  [Arity Op] [PCM T]
+  [DecidableEq χ]
+  [InterpConsts V]
+  {opSpec : OpSpec Op V T}
+  {s s' : ConfigWithSpec opSpec χ m n}
+  {l : Label Op V m n}
+  (hl : l.isYield ∨ l.isSilent)
+  (hstep : (Config.IdxTrivStep opSpec).Step s (i, l) s') :
+    (Config.TrivStep opSpec) s l s'
+  := by
+  rcases hstep with ⟨⟨hguard⟩, hstep⟩
+  cases hguard <;> simp at hl
+  case triv_yield =>
+    have := Config.IndexedStep.to_step_yield_or_tau hstep
+    exact .step .triv_yield this
+  case triv_join =>
+    have := Config.IndexedStep.to_step_yield_or_tau hstep
+    exact .step .triv_join this
+  case triv_tau =>
+    have := Config.IndexedStep.to_step_yield_or_tau hstep
+    exact .step .triv_tau this
+
+/-- Converts an unguarded step to an indexed unguarded step. -/
+theorem proc_unguarded_step_to_indexed_unguarded_step
+  [Arity Op] [PCM T]
+  [DecidableEq χ]
+  [InterpConsts V]
+  {opSpec : OpSpec Op V T}
+  {s s' : ConfigWithSpec opSpec χ m n}
+  {l : Label Op V m n}
+  (hl : l.isYield ∨ l.isSilent)
+  (hstep : (Config.TrivStep opSpec) s l s') :
+    ∃ i, (Config.IdxTrivStep opSpec).Step s (i, l) s'
+  := by
+  cases hstep with | step hguard hstep
+  cases hguard <;> simp at hl
+  case step.triv_yield =>
+    have ⟨i, hstep'⟩ := Config.IndexedStep.from_step_yield hstep
+    exact ⟨i, .step (.idx_guard .triv_yield) hstep'⟩
+  case step.triv_join =>
+    have ⟨i, hstep'⟩ := Config.IndexedStep.from_step_yield hstep
+    exact ⟨i, .step (.idx_guard .triv_join) hstep'⟩
+  case step.triv_tau =>
+    have ⟨i, hstep'⟩ := Config.IndexedStep.from_step_tau hstep
+    exact ⟨i, .step (.idx_guard .triv_tau) hstep'⟩
+
+theorem proc_indexed_guarded_step_to_unguarded
+  [Arity Op] [PCM T]
+  [DecidableEq χ]
+  [InterpConsts V]
+  {opSpec : OpSpec Op V T}
+  {ioSpec : IOSpec V T m n}
+  {s s' : ConfigWithSpec opSpec χ m n}
+  {l : Label Op V m n} :
+    (Config.IdxGuardStep opSpec ioSpec).Step s (i, l) s' →
+    (Config.IdxTrivStep opSpec).Step s (i, l) s'
+  := Guard.map_guard (λ ⟨hguard⟩ => ⟨OpSpec.spec_guard_implies_triv_guard hguard⟩)
+
+theorem proc_indexed_interp_guarded_step_to_unguarded
+  [Arity Op] [PCM T]
+  [DecidableEq χ]
+  [InterpConsts V]
+  [opInterp : OpInterp Op V]
+  {opSpec : OpSpec Op V T}
+  {ioSpec : IOSpec V T m n}
+  {s s' : ConfigWithSpec opSpec χ m n × opInterp.S} :
+    (Config.IdxInterpGuardStep opSpec ioSpec).Step s (i, l) s' →
+    (Config.IdxInterpTrivStep opSpec).Step s (i, l) s'
+  := Lts.IndexedInterpStep.map_step proc_indexed_guarded_step_to_unguarded
+
+theorem proc_indexed_interp_guarded_trace_to_unguarded
+  [Arity Op] [PCM T] [PCM.Lawful T]
+  [DecidableEq χ]
+  [InterpConsts V]
+  [opInterp : OpInterp Op V]
+  {opSpec : OpSpec Op V T}
+  {ioSpec : IOSpec V T m n}
+  {s s' : ConfigWithSpec opSpec χ m n × opInterp.S}
+  (htrace : (Config.IdxInterpGuardStep opSpec ioSpec).Star s tr s') :
+    (Config.IdxInterpTrivStep opSpec).Star s tr s'
+  := htrace.map_step proc_indexed_interp_guarded_step_to_unguarded
+
+end Wavelet.Determinacy
