Wavelet/Semantics.lean
@@ -2,9 +2,7 @@ import Wavelet.Semantics.Defs
 import Wavelet.Semantics.Lts
 import Wavelet.Semantics.Link
 import Wavelet.Semantics.OpInterp
-import Wavelet.Semantics.PCM
 import Wavelet.Semantics.Confluence
 import Wavelet.Semantics.Guard
-import Wavelet.Semantics.OpSpec
 
 /-! Common definitions for semantics. -/
